Warm-up 01
================
Pinshuo Ye
9/7/2017

**Cooking recipe of the Pumpkin Chocolate Chip Cookies**
--------------------------------------------------------

##### "If you like pumpkin pie and chocolate, you'll love these cookies. I think they taste best when they are cold from the refrigerator."

### **Ingredients**

-   1 cup **canned pumpkin**
-   1 cup **white sugar**
-   $\\frac{1}{2}$ cup **vegetable oil**
-   1 **egg**
-   2 cups **all-purpose flour**
-   2 teaspoons **baking powder**
-   2 teaspoons **ground cinnamon**
-   $\\frac{1}{2}$ teaspoon **salt**
-   1 teaspoon **baking soda**
-   1 teaspoon **milk**
-   1 tablespoon **vanilla extract**
-   2 cups semisweet **chocolate chips**
-   $\\frac{1}{2}$ cup chopped **walnuts** *(optional)*

### **Special Kitchen Tools**

-   Bowls
-   Cookie sheet

### **Steps**

1.  Combine pumpkin, sugar, vegetable oil, and egg.
2.  In a separate bowl, stir together flour, baking powder, ground cinnamon, and salt.
3.  Dissolve the baking soda with the milk and stir in.
4.  Add flour mixture to pumpkin mixture and ***mix well***.
5.  Add vanilla, chocolate chips and nuts.
6.  Drop by spoonful on greased cookie sheet and bake at ***350 degrees F (175 degrees C)*** for approximately 10 minutes or until lightly brown and firm.
7.  Done!

![The cookies](http://images.media-allrecipes.com/userphotos/600x600/4524544.jpg)

![The cookies](http://images.media-allrecipes.com/userphotos/600x600/473562.jpg)

##### Now you are finished! Having fun and enjoy your cookies!

##### Here is the link to the original [cookie recipe](http://allrecipes.com/recipe/10740/pumpkin-chocolate-chip-cookies-iii/?clickId=right%20rail%200&internalSource=rr_feed_recipe&referringId=10011&referringContentType=recipe).

**Quadratic Equation**
----------------------

$x=\\frac{-b\\pm\\sqrt{b^2-4ac}}{2a}$

Here are some other equations

*F* = *m**a*

$tan(\\alpha+\\beta)=\\frac{tan(\\alpha)+tan(\\beta)}{1-tan(\\alpha)tan(\\beta)}$

*e*<sup>*i**π*</sup> + 1 = 0

$\\frac{d}{dx}(\\frac{f(x)}{g(x)})=\\frac{g(x)\\frac{d}{dx}f(x)-f(x)\\frac{d}{dx}g(x)}{(g(x))^2}$
